Clean/Halo2.lean
@@ -9,6 +9,7 @@ import Clean.Halo2.Basic
 import Clean.Halo2.Lemmas
 import Clean.Halo2.Loops
 import Clean.Halo2.Formal
+import Clean.Halo2.Keygen
 import Clean.Halo2.Tactics.ProvableTypeSimp
 import Clean.Halo2.Tactics.ContractBridges
 import Clean.Halo2.Tactics.CircuitProofStart2
